backend/RTLtyping.v
@@ -985,7 +985,7 @@ Proof.
 Qed.
 
 Lemma wt_initial_state id sg args m:
-  forall S, initial_state p (id, sg, args, m) S -> wt_state (sig_res sg) S.
+  forall S, initial_state p (cq id sg args m) S -> wt_state (sig_res sg) S.
 Proof.
   intros. inv H. constructor. constructor. auto.
   pattern f. apply Genv.find_funct_ptr_prop with fundef unit p b.
